feat: Calculus

Logic/FirstOrder/Basic/Calculus.lean
@@ -1,56 +1,52 @@
+import Logic.Logic.Calculus
 import Logic.FirstOrder.Basic.Formula
 
 namespace LO
 
 namespace FirstOrder
 
-abbrev Sequent (L : Language.{u}) := Finset (SyntacticFormula L)
+abbrev Sequent (L : Language) := List (SyntacticFormula L)
 
 open Subformula
-variable {L : Language.{u}} [∀ k, DecidableEq (L.Func k)] [∀ k, DecidableEq (L.Rel k)]
+variable {L : Language}
 
-def shifts (Δ : Finset (SyntacticSubformula L n)) :
-  Finset (SyntacticSubformula L n) := Δ.map shiftEmb
+def shifts (Δ : List (SyntacticSubformula L n)) :
+  List (SyntacticSubformula L n) := Δ.map Rew.shift.hom
 
-lemma shifts_eq_image (Δ : Finset (SyntacticSubformula L n)) : shifts Δ = Δ.image Rew.shift.hom := Finset.map_eq_image _ _
+local postfix:max "⁺" => shifts
 
-@[simp] lemma mem_shifts_iff {p : SyntacticSubformula L n} {Δ : Finset (SyntacticSubformula L n)} :
-    Rew.shift.hom p ∈ shifts Δ ↔ p ∈ Δ :=
-  Finset.mem_map' _
+@[simp] lemma mem_shifts_iff {p : SyntacticSubformula L n} {Δ : List (SyntacticSubformula L n)} :
+    Rew.shift.hom p ∈ Δ⁺ ↔ p ∈ Δ :=
+  List.mem_map_of_injective Rew.shift.hom_injective
 
-@[simp] lemma shifts_ss (Δ Γ : Finset (SyntacticSubformula L n)) :
-    shifts Δ ⊆ shifts Γ ↔ Δ ⊆ Γ := Finset.map_subset_map
+@[simp] lemma shifts_ss (Δ Γ : List (SyntacticSubformula L n)) :
+    Δ⁺ ⊆ Γ⁺ ↔ Δ ⊆ Γ := List.map_subset_iff _ Rew.shift.hom_injective
 
-lemma shifts_insert (p : SyntacticSubformula L n) (Δ : Finset (SyntacticSubformula L n)) :
-    shifts (insert p Δ) = insert (Rew.shift.hom p) (shifts Δ) :=
-  by simp[shifts, shiftEmb_eq_shift]
+lemma shifts_insert (p : SyntacticSubformula L n) (Δ : List (SyntacticSubformula L n)) :
+    (p :: Δ)⁺ = Rew.shift.hom p :: Δ⁺ := by simp[shifts]
 
-lemma shifts_union (Δ Γ : Finset (SyntacticSubformula L n)) :
-    shifts (Δ ∪ Γ) = (shifts Δ) ∪ (shifts Γ) :=
-  by simp[shifts, shiftEmb_eq_shift, Finset.map_union]
+lemma shifts_union (Δ Γ : List (SyntacticSubformula L n)) :
+    (Δ ++ Γ)⁺ = Δ⁺ ++ Γ⁺ := by simp[shifts]
 
-@[simp] lemma shifts_emb (s : Finset (Subsentence L n)) :
-    shifts (s.image Rew.emb.hom) = s.image Rew.emb.hom := by
-  simp[shifts, shiftEmb, Finset.map_eq_image, Finset.image_image, Function.comp, ←Rew.hom_comp_app]
-
-lemma shifts_erase (p : SyntacticSubformula L n) (Δ : Finset (SyntacticSubformula L n)) :
-    shifts (Δ.erase p) = (shifts Δ).erase (Rew.shift.hom p) :=
-  by simp[shifts, shiftEmb_eq_shift]
+@[simp] lemma shifts_emb (Γ : List (Subsentence L n)) :
+    (Γ.map Rew.emb.hom)⁺ = Γ.map Rew.emb.hom := by
+  simp[shifts, Function.comp, ←Rew.hom_comp_app]
 
 inductive DerivationCR (P : SyntacticFormula L → Prop) : Sequent L → Type u
-| axL   : ∀ (Δ : Sequent L) {k} (r : L.Rel k) (v : Fin k → SyntacticTerm L),
-    rel r v ∈ Δ → nrel r v ∈ Δ → DerivationCR P Δ
-| verum : ∀ (Δ : Sequent L), ⊤ ∈ Δ → DerivationCR P Δ
-| or    : ∀ (Δ : Sequent L) (p q : SyntacticFormula L),
-    DerivationCR P (insert p $ insert q Δ) → DerivationCR P (insert (p ⋎ q) Δ)
-| and   : ∀ (Δ : Sequent L) (p q : SyntacticFormula L),
-    DerivationCR P (insert p Δ) → DerivationCR P (insert q Δ) → DerivationCR P (insert (p ⋏ q) Δ)
-| all   : ∀ (Δ : Sequent L) (p : SyntacticSubformula L 1),
-    DerivationCR P (insert (Rew.free.hom p) (shifts Δ)) → DerivationCR P (insert (∀' p) Δ)
-| ex    : ∀ (Δ : Sequent L) (t : SyntacticTerm L) (p : SyntacticSubformula L 1),
-    DerivationCR P (insert ([→ t].hom p) Δ) → DerivationCR P (insert (∃' p) Δ)
-| cut   : ∀ (Δ Γ : Sequent L) (p : SyntacticFormula L), P p →
-    DerivationCR P (insert p Δ) → DerivationCR P (insert (~p) Γ) → DerivationCR P (Δ ∪ Γ)
+| axL (Δ) {k} (r : L.Rel k) (v) :
+    DerivationCR P (rel r v :: nrel r v :: Δ)
+| verum (Δ) : DerivationCR P (⊤ :: Δ)
+| or {Δ p q} :
+    DerivationCR P (p :: q :: Δ) → DerivationCR P (p ⋎ q :: Δ)
+| and {Δ p q} :
+    DerivationCR P (p :: Δ) → DerivationCR P (q :: Δ) → DerivationCR P (p ⋏ q :: Δ)
+| all {Δ p} :
+    DerivationCR P (Rew.free.hom p :: Δ⁺) → DerivationCR P ((∀' p) :: Δ)
+| ex {Δ p} (t) :
+    DerivationCR P (p/[t] :: Δ) → DerivationCR P ((∃' p) :: Δ)
+| wk {Δ Γ} : DerivationCR P Δ → Δ ⊆ Γ → DerivationCR P Γ
+| cut {Δ p} : P p →
+    DerivationCR P (p :: Δ) → DerivationCR P (~p :: Δ) → DerivationCR P Δ
 
 scoped notation :45 "⊢ᶜ[" P "] " Γ:45 => DerivationCR P Γ
 
@@ -66,41 +62,41 @@ abbrev DerivationClx (c : ℕ) : Sequent L → Type u := DerivationCR (·.comple
 
 scoped notation :45 "⊢ᶜ[< " c "] " Γ:45 => DerivationClx c Γ
 
-abbrev DerivationList (G : List (SyntacticFormula L)) := ⊢ᶜ G.toFinset
-
-abbrev Derivation₁ (p : SyntacticFormula L) := ⊢ᶜ ({p} : Sequent L)
-
-abbrev Derivation.Valid (σ : Sentence L) := ⊢ᵀ ({Rew.emb.hom σ} : Sequent L)
+instance : OneSided (Sentence L) := ⟨fun Γ ↦ ⊢ᶜ Γ.map Rew.emb.hom⟩
 
 namespace DerivationCR
-variable {P : SyntacticFormula L → Prop} {Δ Δ₁ Δ₂ Γ : Sequent L}
+variable {P : SyntacticFormula L → Prop} {Δ Δ₁ Δ₂ Γ : Sequent L} {p q r : SyntacticFormula L}
 
 def length : {Δ : Sequent L} → DerivationCR P Δ → ℕ
-  | _, axL Δ _ _ _ _     => 0
-  | _, verum Δ _         => 0
-  | _, or _ _ _ d        => d.length.succ
-  | _, and _ _ _ dp dq   => (max dp.length dq.length).succ
-  | _, all _ _ d         => d.length.succ
-  | _, ex _ _ _ d        => d.length.succ
-  | _, cut _ _ _ _ dp dn => (max dp.length dn.length).succ
+  | _, axL _ _ _   => 0
+  | _, verum _     => 0
+  | _, or d        => d.length.succ
+  | _, and dp dq   => (max dp.length dq.length).succ
+  | _, all d       => d.length.succ
+  | _, ex _ d      => d.length.succ
+  | _, wk d _      => d.length.succ
+  | _, cut _ dp dn => (max dp.length dn.length).succ
 
 section
 
-@[simp] lemma length_axL {k} {r : L.Rel k} {v} (hpos : rel r v ∈ Δ) (hneg : nrel r v ∈ Δ) :
-  (axL (P := P) Δ r v hpos hneg).length = 0 := rfl
+@[simp] lemma length_axL {k} {r : L.Rel k} {v} :
+  (axL (P := P) Δ r v).length = 0 := rfl
 
-@[simp] lemma length_verum (h : ⊤ ∈ Δ) : (verum (P := P) Δ h).length = 0 := rfl
+@[simp] lemma length_verum : (verum (P := P) Δ).length = 0 := rfl
 
-@[simp] lemma length_and {p q} (dp : ⊢ᶜ[P] insert p Δ) (dq : ⊢ᶜ[P] insert q Δ) : (and Δ p q dp dq).length = (max dp.length dq.length).succ := rfl
+@[simp] lemma length_and {p q} (dp : ⊢ᶜ[P] p :: Δ) (dq : ⊢ᶜ[P] q :: Δ) :
+    (and dp dq).length = (max dp.length dq.length).succ := rfl
 
-@[simp] lemma length_or {p q} (d : ⊢ᶜ[P] (insert p $ insert q Δ)) : (or Δ p q d).length = d.length.succ := rfl
+@[simp] lemma length_or {p q} (d : ⊢ᶜ[P] (p :: q :: Δ)) : (or d).length = d.length.succ := rfl
 
-@[simp] lemma length_all {p} (d : ⊢ᶜ[P] insert (Rew.free.hom p) (shifts Δ)) : (all Δ p d).length = d.length.succ := rfl
+@[simp] lemma length_all {p} (d : ⊢ᶜ[P] Rew.free.hom p :: Δ⁺) : (all d).length = d.length.succ := rfl
 
-@[simp] lemma length_ex {t} {p} (d : ⊢ᶜ[P] insert ([→ t].hom p) Δ) : (ex Δ t p d).length = d.length.succ := rfl
+@[simp] lemma length_ex {t} {p} (d : ⊢ᶜ[P] p/[t] :: Δ) : (ex t d).length = d.length.succ := rfl
 
-@[simp] lemma length_cut {p} (hp : P p) (dp : ⊢ᶜ[P] insert p Δ) (dn : ⊢ᶜ[P] insert (~p) Γ) :
-  (cut _ _ p hp dp dn).length = (max dp.length dn.length).succ := rfl
+@[simp] lemma length_wk (d : ⊢ᶜ[P] Δ) (h : Δ ⊆ Γ) : (wk d h).length = d.length.succ := rfl
+
+@[simp] lemma length_cut {p} (hp : P p) (dp : ⊢ᶜ[P] p :: Δ) (dn : ⊢ᶜ[P] (~p) :: Δ) :
+  (cut hp dp dn).length = (max dp.length dn.length).succ := rfl
 
 end
 
@@ -108,55 +104,66 @@ section Repr
 variable [∀ k, ToString (L.Func k)] [∀ k, ToString (L.Rel k)]
 
 protected unsafe def repr : {Δ : Sequent L} → ⊢ᶜ[P] Δ → String
-  | _, axL Δ _ _ _ _   =>
+  | _, axL Δ _ _   =>
       "\\AxiomC{}\n" ++
       "\\RightLabel{\\scriptsize(axL)}\n" ++
       "\\UnaryInfC{$" ++ reprStr Δ ++ "$}\n\n"
-  | _, verum Δ _       =>
+  | _, verum Δ       =>
       "\\AxiomC{}\n" ++
       "\\RightLabel{\\scriptsize($\\top$)}\n" ++
       "\\UnaryInfC{$" ++ reprStr Δ ++ "$}\n\n"
-  | _, or Δ p q d      =>
+  | _, @or _ _ Δ p q d      =>
       d.repr ++
       "\\RightLabel{\\scriptsize($\\lor$)}\n" ++
-      "\\UnaryInfC{$" ++ reprStr (insert (p ⋎ q) Δ) ++ "$}\n\n"
-  | _, and Δ p q dp dq =>
+      "\\UnaryInfC{$" ++ reprStr ((p ⋎ q) :: Δ) ++ "$}\n\n"
+  | _, @and _ _ Δ p q dp dq =>
       dp.repr ++
       dq.repr ++
       "\\RightLabel{\\scriptsize($\\land$)}\n" ++
-      "\\BinaryInfC{$" ++ reprStr (insert (p ⋏ q) Δ) ++ "$}\n\n"
-  | _, all Δ p d       =>
+      "\\BinaryInfC{$" ++ reprStr ((p ⋏ q) :: Δ) ++ "$}\n\n"
+  | _, @all _ _ Δ p d       =>
       d.repr ++
       "\\RightLabel{\\scriptsize($\\forall$)}\n" ++
-      "\\UnaryInfC{$" ++ reprStr (insert (∀' p) Δ) ++ "$}\n\n"
-  | _, ex Δ _ p d      =>
+      "\\UnaryInfC{$" ++ reprStr ((∀' p) :: Δ) ++ "$}\n\n"
+  | _, @ex _ _ Δ p _ d      =>
       d.repr ++
       "\\RightLabel{\\scriptsize($\\exists$)}\n" ++
-      "\\UnaryInfC{$" ++ reprStr (insert (∃' p) Δ) ++ "$}\n\n"
-  | _, cut Δ Γ _ _ dp dn =>
+      "\\UnaryInfC{$" ++ reprStr ((∃' p) :: Δ) ++ "$}\n\n"
+  | _, @wk _ _ _ Γ d _      =>
+      d.repr ++
+      "\\RightLabel{\\scriptsize(wk)}\n" ++
+      "\\UnaryInfC{$" ++ reprStr Γ ++ "$}\n\n"
+  | _, @cut _ _ Δ _ _ dp dn =>
       dp.repr ++
       dn.repr ++
       "\\RightLabel{\\scriptsize(Cut)}\n" ++
-      "\\BinaryInfC{$" ++ reprStr (Δ ∪ Γ) ++ "$}\n\n"
+      "\\BinaryInfC{$" ++ reprStr Δ ++ "$}\n\n"
 
 unsafe instance : Repr (⊢ᶜ[P] Δ) where reprPrec d _ := d.repr
 
 end Repr
 
-protected def cast (d : ⊢ᶜ[P] Δ) (e : Δ = Γ) : ⊢ᶜ[P] Γ := cast (by simp[HasVdash.vdash, e]) d
+protected abbrev cast (d : ⊢ᶜ[P] Δ) (e : Δ = Γ) : ⊢ᶜ[P] Γ := cast (congrArg (DerivationCR P) e) d
 
 def cast₀ (d : ⊢ᵀ Δ) (e : Δ = Γ) : ⊢ᵀ Γ := d.cast e
 
-@[simp] lemma length_cast (d : ⊢ᶜ[P] Δ) (e : Δ = Γ) : (d.cast e).length = d.length := by rcases e with rfl; simp[DerivationCR.cast]
+@[simp] lemma cast_eq (d : ⊢ᶜ[P] Δ) (e : Δ = Δ) : d.cast e = d := rfl
+
+@[simp] lemma length_cast (d : ⊢ᶜ[P] Δ) (e : Δ = Γ) :
+    (d.cast e).length = d.length := by rcases e with rfl; simp[DerivationCR.cast]
+
+@[simp] lemma length_cast' (d : ⊢ᶜ[P] Δ) (e : Δ = Γ) :
+    (cast (congrArg (DerivationCR P) e) d).length = d.length := by rcases e with rfl; simp[DerivationCR.cast]
 
 def cutWeakening {P Q : SyntacticFormula L → Prop} (h : ∀ p, P p → Q p) : ∀ {Δ}, ⊢ᶜ[P] Δ → ⊢ᶜ[Q] Δ
-  | _, axL Δ r v hpos hneg  => axL Δ r v hpos hneg
-  | _, verum Δ h            => verum Δ h
-  | _, and Δ p q dp dq      => and Δ p q (dp.cutWeakening h) (dq.cutWeakening h)
-  | _, or Δ p q d           => or Δ p q (d.cutWeakening h)
-  | _, all Δ p d            => all Δ p (d.cutWeakening h)
-  | _, ex Δ t p d           => ex Δ t p (d.cutWeakening h)
-  | _, cut Δ₁ Δ₂ p hp d₁ d₂ => cut Δ₁ Δ₂ p (h p hp) (d₁.cutWeakening h) (d₂.cutWeakening h)
+  | _, axL Δ r v    => axL Δ r v
+  | _, verum Δ      => verum Δ
+  | _, and dp dq    => and (dp.cutWeakening h) (dq.cutWeakening h)
+  | _, or d         => or (d.cutWeakening h)
+  | _, all d        => all (d.cutWeakening h)
+  | _, ex t d       => ex t (d.cutWeakening h)
+  | _, wk d ss      => wk (d.cutWeakening h) ss
+  | _, cut hp d₁ d₂ => cut (h _ hp) (d₁.cutWeakening h) (d₂.cutWeakening h)
 
 @[simp] lemma lengtgh_cutWeakening {P Q : SyntacticFormula L → Prop} (h : ∀ p, P p → Q p) {Δ} (d : ⊢ᶜ[P] Δ) :
     (d.cutWeakening h).length = d.length := by induction d <;> simp[*, cutWeakening]
@@ -165,52 +172,17 @@ def ofLe {i j : ℕ} (h : i ≤ j) : ⊢ᶜ[< i] Δ → ⊢ᶜ[< j] Δ := cutWea
 
 def cutWeakeningCut (d : ⊢ᶜ[P] Δ) : ⊢ᶜ Δ := d.cutWeakening (by simp)
 
-def weakening : ∀ {Δ}, ⊢ᶜ[P] Δ → ∀ {Γ : Sequent L}, Δ ⊆ Γ → ⊢ᶜ[P] Γ
-  | _, axL Δ r v hrel hnrel, Γ, h => axL Γ r v (h hrel) (h hnrel)
-  | _, verum Δ htop,         Γ, h => verum Γ (h htop)
-  | _, or Δ p q d,           Γ, h =>
-      have : ⊢ᶜ[P] (insert p $ insert q Γ) :=
-        weakening d (Finset.insert_subset_insert p $ Finset.insert_subset_insert q (Finset.insert_subset_iff.mp h).2)
-      have : ⊢ᶜ[P] insert (p ⋎ q) Γ := or Γ p q this
-      this.cast (by simp; exact (Finset.insert_subset_iff.mp h).1)
-  | _, and Δ p q dp dq,      Γ, h =>
-      have dp : ⊢ᶜ[P] insert p Γ := dp.weakening (Finset.insert_subset_insert p (Finset.insert_subset_iff.mp h).2)
-      have dq : ⊢ᶜ[P] insert q Γ := dq.weakening (Finset.insert_subset_insert q (Finset.insert_subset_iff.mp h).2)
-      have : ⊢ᶜ[P] insert (p ⋏ q) Γ := and Γ p q dp dq
-      this.cast (by simp; exact (Finset.insert_subset_iff.mp h).1)
-  | _, all Δ p d,            Γ, h =>
-      have : ⊢ᶜ[P] insert (Rew.free.hom p) (shifts Γ) := d.weakening (Finset.insert_subset_insert _ $ by simpa using (Finset.insert_subset_iff.mp h).2)
-      have : ⊢ᶜ[P] insert (∀' p) Γ := all Γ p this
-      this.cast (by simp; exact (Finset.insert_subset_iff.mp h).1)
-  | _, ex Δ t p d,           Γ, h =>
-      have : ⊢ᶜ[P] insert ([→ t].hom p) Γ := d.weakening (Finset.insert_subset_insert _ $ by simpa using (Finset.insert_subset_iff.mp h).2)
-      have : ⊢ᶜ[P] insert (∃' p) Γ := ex Γ t p this
-      this.cast (by simp; exact (Finset.insert_subset_iff.mp h).1)
-  | _, cut Δ₁ Δ₂ p hp d₁ d₂, Γ, h =>
-      have d₁ : ⊢ᶜ[P] insert p Γ := d₁.weakening (Finset.insert_subset_insert _ (Finset.union_subset_left h))
-      have d₂ : ⊢ᶜ[P] insert (~p) Γ := d₂.weakening (Finset.insert_subset_insert _ (Finset.union_subset_right h))
-      (cut Γ Γ p hp d₁ d₂).cast (by simp)
+alias weakening := wk
 
-@[simp] lemma length_weakening {Δ} (d : ⊢ᶜ[P] Δ) {Γ : Sequent L} (h : Δ ⊆ Γ) : (d.weakening h).length = d.length :=
-  by induction d generalizing Γ <;> simp[*, weakening]
+def verum' (h : ⊤ ∈ Δ) : ⊢ᶜ[P] Δ := (verum Δ).wk (by simp[h])
 
-def or' {p q : SyntacticFormula L} (h : p ⋎ q ∈ Δ) (d : ⊢ᶜ[P] (insert p $ insert q $ Δ.erase (p ⋎ q))) : ⊢ᶜ[P] Δ :=
-  (or _ p q d).cast (by simp[Finset.insert_erase h])
+def axL' {k} (r : L.Rel k) (v)
+    (h : Subformula.rel r v ∈ Δ) (hn : Subformula.nrel r v ∈ Δ) : ⊢ᶜ[P] Δ := (axL Δ r v).wk (by simp[h, hn])
 
-def and' {p q : SyntacticFormula L} (h : p ⋏ q ∈ Δ) (dp : ⊢ᶜ[P] insert p (Δ.erase (p ⋏ q))) (dq : ⊢ᶜ[P] insert q (Δ.erase (p ⋏ q))) : ⊢ᶜ[P] Δ :=
-  (and _ p q dp dq).cast (by simp[Finset.insert_erase h])
+def cCut (d₁ : ⊢ᶜ p :: Δ) (d₂ : ⊢ᶜ ~p :: Δ) : ⊢ᶜ Δ := cut trivial d₁ d₂
 
-def all' {p : SyntacticSubformula L 1} (h : ∀' p ∈ Δ) (d : ⊢ᶜ[P] insert (Rew.free.hom p) (shifts $ Δ.erase (∀' p))) : ⊢ᶜ[P] Δ :=
-  (all _ p d).cast (by simp[Finset.insert_erase h])
-
-def ex' {p : SyntacticSubformula L 1} (t : SyntacticTerm L) (h : ∃' p ∈ Δ)
-  (d : ⊢ᶜ[P] insert ([→ t].hom p) (Δ.erase (∃' p))) : ⊢ᶜ[P] Δ :=
-  (ex _ t p d).cast (by simp[Finset.insert_erase h])
-
-def cCut {p} (d₁ : ⊢ᶜ insert p Δ) (d₂ : ⊢ᶜ insert (~p) Γ) : ⊢ᶜ Δ ∪ Γ := cut Δ Γ p trivial d₁ d₂
-
-def cutClx {i} {p} (d₁ : ⊢ᶜ[< i] insert p Δ) (d₂ : ⊢ᶜ[< i] insert (~p) Γ) (hp : p.complexity < i) :
-    ⊢ᶜ[< i] Δ ∪ Γ := cut Δ Γ p hp d₁ d₂
+def cutClx {i p} (d₁ : ⊢ᶜ[< i] p :: Δ) (d₂ : ⊢ᶜ[< i] ~p :: Δ) (hp : p.complexity < i) :
+    ⊢ᶜ[< i] Δ := cut hp d₁ d₂
 
 @[simp] lemma ne_step_max (n m : ℕ) : n ≠ max n m + 1 :=
   ne_of_lt $ Nat.lt_succ_of_le $ by simp
@@ -222,55 +194,41 @@ private lemma neg_ne_and {p q : SyntacticFormula L} : ¬~p = p ⋏ q :=
 ne_of_ne_complexity (by simp)
 
 def em {p : SyntacticFormula L} {Δ : Sequent L} (hpos : p ∈ Δ) (hneg : ~p ∈ Δ) : ⊢ᶜ[P] Δ := by
-  induction p using Subformula.formulaRec generalizing Δ
-  case hverum           => exact verum Δ hpos
-  case hfalsum          => exact verum Δ hneg
-  case hrel r v         => exact axL Δ r v hpos hneg
-  case hnrel r v        => exact axL Δ r v hneg hpos
+  induction p using Subformula.formulaRec generalizing Δ <;> simp at hneg
+  case hverum           => exact verum' hpos
+  case hfalsum          => exact verum' hneg
+  case hrel r v         => exact axL' r v hpos hneg
+  case hnrel r v        => exact axL' r v hneg hpos
   case hall p ih        =>
-    exact all' hpos $ ex' (p := ~Rew.shift.hom p) &0
-      (by simp; exact Or.inr (by simp[shifts, shiftEmb_eq_shift]; exact ⟨_, hneg, by simp⟩))
-      (ih (by simp; exact Or.inr $ ne_of_ne_complexity $ by simp[Rew.shift]) (by simp))
+    have : ⊢ᶜ[P] ~Rew.free.hom p :: Rew.free.hom p :: Δ⁺ := ih (by simp) (by simp)
+    have : ⊢ᶜ[P] (~Rew.shift.hom p)/[&0] :: Rew.free.hom p :: Δ⁺ :=
+      this.cast (by simp[←Rew.hom_comp_app])
+    have : ⊢ᶜ[P] Rew.free.hom p :: Δ⁺ := (ex &0 this).wk
+      (by simp; right;
+          have := mem_shifts_iff.mpr hneg
+          rwa [Rew.ex, Rew.q_shift, LogicSymbol.HomClass.map_neg] at this)
+    exact this.all.wk (by simp[hpos])
   case hex p ih         =>
-    simp at hneg
-    exact all' hneg $ ex' (p := Rew.shift.hom p) &0
-      (by simp; exact Or.inr (by simp[shifts, shiftEmb_eq_shift]; exact ⟨_, hpos, by simp⟩))
-      (ih (by simp) (by simp; exact Or.inr $ ne_of_ne_complexity $ by simp[Rew.shift]))
+    have : ⊢ᶜ[P] Rew.free.hom p :: ~Rew.free.hom p :: Δ⁺ := ih (by simp) (by simp)
+    have : ⊢ᶜ[P] (Rew.shift.hom p)/[&0] :: ~Rew.free.hom p :: Δ⁺ :=
+      this.cast (by simp[←Rew.hom_comp_app])
+    have : ⊢ᶜ[P] Rew.free.hom (~p) :: Δ⁺ := (ex &0 this).wk
+      (by simp; right;
+          have := mem_shifts_iff.mpr hpos
+          rwa [Rew.ex, Rew.q_shift] at this)
+    exact this.all.wk (by simp[hneg])
   case hand p q ihp ihq =>
-    simp at hneg
-    exact or' hneg (and' (p := p) (q := q) (by simp[hpos])
-      (ihp (by simp) (by simp; exact Or.inr $ ne_of_ne_complexity (by simp)))
-      (ihq (by simp) (by simp; exact Or.inr $ ne_of_ne_complexity (by simp))))
+    have ihp : ⊢ᶜ[P] p :: ~p :: ~q :: Δ := ihp (by simp) (by simp)
+    have ihq : ⊢ᶜ[P] q :: ~p :: ~q :: Δ := ihq (by simp) (by simp)
+    have : ⊢ᶜ[P] ~p :: ~q :: Δ := (ihp.and ihq).wk (by simp[hpos])
+    exact this.or.wk (by simp[hneg])
   case hor p q ihp ihq  =>
-    simp at hneg
-    exact or' hpos (and' (p := ~p) (q := ~q) (by simp[hneg])
-      (ihp (by simp; exact Or.inr $ ne_of_ne_complexity (by simp)) (by simp))
-      (ihq (by simp; exact Or.inr $ ne_of_ne_complexity (by simp)) (by simp)))
+    have ihp : ⊢ᶜ[P] ~p :: p :: q :: Δ := ihp (by simp) (by simp)
+    have ihq : ⊢ᶜ[P] ~q :: p :: q :: Δ := ihq (by simp) (by simp)
+    have : ⊢ᶜ[P] p :: q :: Δ := (ihp.and ihq).wk (by simp[hneg])
+    exact this.or.wk (by simp[hpos])
 
-def elimFalsum : {Δ : Sequent L} → ⊢ᶜ[P] Δ → ⊢ᶜ[P] Δ.erase ⊥
-  | _, axL Δ r v hpos hneg => axL _ r v (by simp[hpos]) (by simp[hneg])
-  | _, verum Δ h           => verum _ (by simp[h])
-  | _, and Δ p q dp dq     =>
-    have dp : ⊢ᶜ[P] insert p (Δ.erase ⊥) := dp.elimFalsum.weakening (by simp[Finset.subset_iff]; rintro x hx (rfl | hhx) <;> simp[*])
-    have dq : ⊢ᶜ[P] insert q (Δ.erase ⊥) := dq.elimFalsum.weakening (by simp[Finset.subset_iff]; rintro x hx (rfl | hhx) <;> simp[*])
-    (and _ p q dp dq).cast (by simp[Finset.erase_insert_of_ne])
-  | _, or Δ p q d          =>
-    have : ⊢ᶜ[P] (insert p $ insert q $ Δ.erase ⊥) :=
-      d.elimFalsum.weakening (by simp[Finset.subset_iff]; rintro x hx (rfl | hhx) <;> simp[*])
-    (or _ _ _ this).cast (by simp[Finset.erase_insert_of_ne])
-  | _, all Δ p d           =>
-    have : ⊢ᶜ[P] (insert (Rew.free.hom p) (shifts $ Δ.erase ⊥)) :=
-      d.elimFalsum.weakening
-        (by {simp[Finset.subset_iff, shifts_eq_image]; rintro x hx (rfl | ⟨y, hy, rfl⟩); { exact Or.inl rfl };
-             { exact Or.inr ⟨y, ⟨by rintro rfl; simp at hx, hy⟩, rfl⟩ } } )
-    (all _ _ this).cast (by simp[Finset.erase_insert_of_ne])
-  | _, ex Δ t p d          =>
-    have : ⊢ᶜ[P] (insert ([→ t].hom p) $ Δ.erase ⊥) := d.elimFalsum.weakening (by simp[Finset.subset_iff]; rintro x hx (rfl | hhx) <;> simp[*])
-    (ex _ t p this).cast (by simp[Finset.erase_insert_of_ne])
-  | _, cut Δ Γ p hp dΔ dΓ  =>
-    have dΔ : ⊢ᶜ[P] (insert p $ Δ.erase ⊥) := dΔ.elimFalsum.weakening (by simp[Finset.subset_iff]; rintro x hx (rfl | hhx) <;> simp[*])
-    have dΓ : ⊢ᶜ[P] (insert (~p) $ Γ.erase ⊥) := dΓ.elimFalsum.weakening (by simp[Finset.subset_iff]; rintro x hx (rfl | hhx) <;> simp[*])
-    (cut _ _ p hp dΔ dΓ).cast (by simp[Finset.erase_union])
+-- def elimFalsum (d : ⊢ᶜ[P] (⊥ :: Δ)) : ⊢ᶜ[P] Δ := by
 
 section Hom
 
@@ -279,41 +237,43 @@ variable
   {L₂ : Language} [∀ k, DecidableEq (L₂.Func k)] [∀ k, DecidableEq (L₂.Rel k)]
   {Δ₁ Γ₁ : Finset (SyntacticFormula L₁)}
 
-lemma shifts_image (Φ : L₁ →ᵥ L₂) {Δ : Finset (SyntacticFormula L₁)} :
-     shifts (Δ.image $ Subformula.lMap Φ) = (Finset.image (Subformula.lMap Φ) (shifts Δ)) :=
+lemma shifts_image (Φ : L₁ →ᵥ L₂) {Δ : List (SyntacticFormula L₁)} :
+     (Δ.map $ .lMap Φ)⁺ = ((Δ⁺).map (.lMap Φ)) :=
   by simp[shifts, shiftEmb, Finset.map_eq_image, Finset.image_image, Function.comp, Subformula.lMap_shift]
 
-def lMap (Φ : L₁ →ᵥ L₂) {P₁ : SyntacticFormula L₁ → Prop} {P₂ : SyntacticFormula L₂ → Prop} (h : ∀ p, P₁ p → P₂ (Subformula.lMap Φ p)):
-    ∀ {Δ : Finset (SyntacticFormula L₁)}, ⊢ᶜ[P₁] Δ → ⊢ᶜ[P₂] Δ.image (Subformula.lMap Φ)
-  | _, axL Δ r v hrel hnrel =>
-      axL _ (Φ.rel r) (fun i => (v i).lMap Φ)
-        (Finset.mem_image_of_mem _ hrel) (Finset.mem_image_of_mem _ hnrel)
-  | _, verum Δ h            => verum _ (by simpa using Finset.mem_image_of_mem (Subformula.lMap Φ) h)
-  | _, or Δ p q d           =>
-      have : ⊢ᶜ[P₂] insert (Subformula.lMap Φ p ⋎ Subformula.lMap Φ q) (Δ.image (Subformula.lMap Φ)) :=
-        or _ _ _ ((d.lMap Φ h).cast (by simp))
+def lMap (Φ : L₁ →ᵥ L₂) {P₁ : SyntacticFormula L₁ → Prop} {P₂ : SyntacticFormula L₂ → Prop}
+    (h : ∀ p, P₁ p → P₂ (.lMap Φ p)):
+    ∀ {Δ}, ⊢ᶜ[P₁] Δ → ⊢ᶜ[P₂] Δ.map (.lMap Φ)
+  | _, axL Δ r v            =>
+      by simp[Subformula.lMap_rel, Subformula.lMap_nrel]; exact axL _ _ _
+  | _, verum Δ              => by simpa using verum _
+  | _, @or _ _ Δ p q d      => by
+      have : ⊢ᶜ[P₂] .lMap Φ p ⋎ .lMap Φ q :: Δ.map (.lMap Φ) :=
+        or (by simpa using d.lMap Φ h)
+      exact this.cast (by simp)
+  | _, @and _ _ Δ p q dp dq =>
+      have : ⊢ᶜ[P₂] .lMap Φ p ⋏ .lMap Φ q :: (Δ.map (.lMap Φ)) :=
+        and ((dp.lMap Φ h).cast (by simp)) ((dq.lMap Φ h).cast (by simp))
       this.cast (by simp)
-  | _, and Δ p q dp dq      =>
-      have : ⊢ᶜ[P₂] insert (Subformula.lMap Φ p ⋏ Subformula.lMap Φ q) (Δ.image (Subformula.lMap Φ)) :=
-        and _ _ _ ((dp.lMap Φ h).cast (by simp)) ((dq.lMap Φ h).cast (by simp))
+  | _, @all _ _ Δ p d       =>
+      have : ⊢ᶜ[P₂] (∀' .lMap Φ p) :: (Δ.map (.lMap Φ)) :=
+        all ((d.lMap Φ h).cast (by simp[←Subformula.lMap_free, shifts_image]))
       this.cast (by simp)
-  | _, all Δ p d            =>
-      have : ⊢ᶜ[P₂] insert (∀' Subformula.lMap Φ p) (Δ.image (Subformula.lMap Φ)) :=
-        all _ _ ((d.lMap Φ h).cast (by simp[←Subformula.lMap_free, shifts_image]))
+  | _, @ex _ _ Δ p t d      =>
+      have : ⊢ᶜ[P₂] (∃' .lMap Φ p) :: (Δ.map (.lMap Φ)) :=
+        ex (Subterm.lMap Φ t)
+          ((d.lMap Φ h).cast (by simp[Subformula.lMap_substs, Matrix.constant_eq_singleton]))
       this.cast (by simp)
-  | _, ex Δ t p d           =>
-      have : ⊢ᶜ[P₂] insert (∃' Subformula.lMap Φ p) (Δ.image (Subformula.lMap Φ)) :=
-        ex _ (Subterm.lMap Φ t) _ ((d.lMap Φ h).cast (by simp[Subformula.lMap_substs, Matrix.constant_eq_singleton]))
-      this.cast (by simp)
-  | _, cut Δ Γ p hp dΔ dΓ   =>
-      have : ⊢ᶜ[P₂] (Δ.image (Subformula.lMap Φ)) ∪ (Γ.image (Subformula.lMap Φ)) :=
-        cut _ _ (Subformula.lMap Φ p) (h p hp) ((dΔ.lMap Φ h).cast (by simp)) ((dΓ.lMap Φ h).cast (by simp))
+  | _, @wk _ _ Δ Γ d ss     => (d.lMap Φ h).wk (List.map_subset _ ss)
+  | _, @cut _ _ Δ p hp d dn =>
+      have : ⊢ᶜ[P₂] (Δ.map (.lMap Φ)) :=
+        cut (h p hp) ((d.lMap Φ h).cast (by simp)) ((dn.lMap Φ h).cast (by simp))
       this.cast (by simp[Finset.image_union])
 
-def lMap₀ (Φ : L₁ →ᵥ L₂) {Δ : Finset (SyntacticFormula L₁)} (d : ⊢ᵀ Δ) : ⊢ᵀ Δ.image (Subformula.lMap Φ) :=
+def lMap₀ (Φ : L₁ →ᵥ L₂) {Δ : Sequent L₁} (d : ⊢ᵀ Δ) : ⊢ᵀ Δ.map (.lMap Φ) :=
   d.lMap Φ (fun _ x => x)
 
-def lMapCut (Φ : L₁ →ᵥ L₂) {Δ : Finset (SyntacticFormula L₁)} (d : ⊢ᶜ Δ) : ⊢ᶜ Δ.image (Subformula.lMap Φ) :=
+def lMapCut (Φ : L₁ →ᵥ L₂) {Δ : Sequent L₁} (d : ⊢ᶜ Δ) : ⊢ᶜ Δ.map (.lMap Φ) :=
   d.lMap Φ (fun _ x => x)
 
 end Hom
@@ -332,359 +292,128 @@ private lemma rewrite_subst_eq (f : ℕ → SyntacticTerm L) (t) (p : SyntacticS
   simp[←Rew.hom_comp_app]; exact Rew.hom_ext' (by ext x <;> simp[Rew.comp_app])
 
 protected def rewrite (h : ∀ f p, P p → P ((Rew.rewrite f).hom p)) :
-    ∀ {Δ : Sequent L}, ⊢ᶜ[P] Δ → ∀ (f : ℕ → SyntacticTerm L), ⊢ᶜ[P] Δ.image ((Rew.rewrite f).hom)
-  | _, axL Δ r v hrel hnrel, f =>
-    axL _ r (fun i => Rew.rewrite f (v i))
-      (by simpa[(Rew.rewrite f).rel] using Finset.mem_image_of_mem ((Rew.rewrite f).hom) hrel)
-      (by simpa[(Rew.rewrite f).nrel] using Finset.mem_image_of_mem ((Rew.rewrite f).hom) hnrel)
-  | _, verum Δ h,            f => verum _ (by simpa using Finset.mem_image_of_mem ((Rew.rewrite f).hom) h)
-  | _, or Δ p q d,           f =>
-    have : ⊢ᶜ[P] insert ((Rew.rewrite f).hom p ⋎ (Rew.rewrite f).hom q) (Δ.image ((Rew.rewrite f).hom)) := or _ _ _ ((d.rewrite h f).cast (by simp))
+    ∀ {Δ : Sequent L}, ⊢ᶜ[P] Δ → ∀ (f : ℕ → SyntacticTerm L), ⊢ᶜ[P] Δ.map (Rew.rewrite f).hom
+  | _, axL Δ r v,            f =>
+    (axL (Δ.map ((Rew.rewrite f).hom)) r (fun x => Rew.rewrite f (v x))).cast
+      (by simp[Rew.rel, Rew.nrel])
+  | _, verum Δ,              f => (verum (Δ.map ((Rew.rewrite f).hom))).cast (by simp)
+  | _, @or _ _ Δ p q d,      f =>
+    have : ⊢ᶜ[P] (Rew.rewrite f).hom p ⋎ (Rew.rewrite f).hom q :: Δ.map ((Rew.rewrite f).hom) :=
+      or ((d.rewrite h f).cast (by simp))
     this.cast (by simp)
-  | _, and Δ p q dp dq,      f =>
-    have : ⊢ᶜ[P] insert ((Rew.rewrite f).hom p ⋏ (Rew.rewrite f).hom q) (Δ.image ((Rew.rewrite f).hom)) := and _ _ _ ((dp.rewrite h f).cast (by simp)) ((dq.rewrite h f).cast (by simp))
+  | _, @and _ _ Δ p q dp dq, f =>
+    have : ⊢ᶜ[P] (Rew.rewrite f).hom p ⋏ (Rew.rewrite f).hom q :: Δ.map ((Rew.rewrite f).hom) :=
+      and ((dp.rewrite h f).cast (by simp)) ((dq.rewrite h f).cast (by simp))
     this.cast (by simp)
-  | _, all Δ p d,            f =>
-    have : ⊢ᶜ[P] (insert (Rew.free.hom p) (shifts Δ)).image (Rew.rewrite (&0 :>ₙ fun x => Rew.shift (f x))).hom := d.rewrite h (&0 :>ₙ fun x => Rew.shift (f x))
-    have : ⊢ᶜ[P] insert (∀' (Rew.rewrite (Rew.bShift ∘ f)).hom p) (Δ.image ((Rew.rewrite f).hom)) :=
-      all _ _ (this.cast (by simp[free_rewrite_eq, shift_rewrite_eq, shifts_eq_image, Finset.image_image, Function.comp]))
+  | _, @all _ _ Δ p d,       f =>
+    have : ⊢ᶜ[P] ((Rew.free.hom p) :: Δ⁺).map (Rew.rewrite (&0 :>ₙ fun x => Rew.shift (f x))).hom :=
+      d.rewrite h (&0 :>ₙ fun x => Rew.shift (f x))
+    have : ⊢ᶜ[P] (∀' (Rew.rewrite (Rew.bShift ∘ f)).hom p) :: Δ.map ((Rew.rewrite f).hom) :=
+      all (this.cast (by simp[free_rewrite_eq, shifts, shift_rewrite_eq, Finset.image_image, Function.comp]))
     this.cast (by simp[Rew.q_rewrite])
-  | _, ex Δ t p d,           f =>
-    have : ⊢ᶜ[P] (insert ([→ t].hom p) Δ).image ((Rew.rewrite f).hom) := d.rewrite h f
-    have : ⊢ᶜ[P] insert (∃' (Rew.rewrite (Rew.bShift ∘ f)).hom p) (Δ.image ((Rew.rewrite f).hom)) :=
-      ex _ (Rew.rewrite f t) _ (this.cast (by simp[rewrite_subst_eq]))
+  | _, @ex _ _ Δ p t d,      f =>
+    have : ⊢ᶜ[P] (p/[t] :: Δ).map ((Rew.rewrite f).hom) := d.rewrite h f
+    have : ⊢ᶜ[P] (∃' (Rew.rewrite (Rew.bShift ∘ f)).hom p) :: Δ.map ((Rew.rewrite f).hom) :=
+      ex (Rew.rewrite f t) (this.cast (by simp[rewrite_subst_eq]))
     this.cast (by simp[Rew.q_rewrite])
-  | _, cut Δ Γ p hp dΔ dΓ,   f =>
-    have dΔ : ⊢ᶜ[P] insert ((Rew.rewrite f).hom p) (Δ.image $ (Rew.rewrite f).hom) := (dΔ.rewrite h f).cast (by simp)
-    have dΓ : ⊢ᶜ[P] insert (~(Rew.rewrite f).hom p) (Γ.image $ (Rew.rewrite f).hom) := (dΓ.rewrite h f).cast (by simp)
-    (cut _ _ ((Rew.rewrite f).hom p) (h f p hp) dΔ dΓ).cast (by simp[Finset.image_union])
+  | _, @wk _ _ Δ Γ d ss,     f => (d.rewrite h f).wk (List.map_subset _ ss)
+  | _, @cut _ _ Δ p hp d dn, f =>
+    have dΔ : ⊢ᶜ[P] ((Rew.rewrite f).hom p) :: Δ.map ((Rew.rewrite f).hom) := (d.rewrite h f).cast (by simp)
+    have dΓ : ⊢ᶜ[P] (~(Rew.rewrite f).hom p) :: Δ.map ((Rew.rewrite f).hom) := (dn.rewrite h f).cast (by simp)
+    (cut (h f p hp) dΔ dΓ).cast (by simp)
 
-def rewrite₀ {Δ : Sequent L} (d : ⊢ᵀ Δ) (f : ℕ → SyntacticTerm L) : ⊢ᵀ Δ.image ((Rew.rewrite f).hom) := d.rewrite (by simp) f
+def rewrite₀ {Δ : Sequent L} (d : ⊢ᵀ Δ) (f : ℕ → SyntacticTerm L) :
+    ⊢ᵀ Δ.map ((Rew.rewrite f).hom) := d.rewrite (by simp) f
 
-def rewriteClx {i} {Δ : Sequent L} (d : ⊢ᶜ[< i] Δ) (f : ℕ → SyntacticTerm L) : ⊢ᶜ[< i] Δ.image ((Rew.rewrite f).hom) := d.rewrite (by simp) f
+def rewriteClx {i} {Δ : Sequent L} (d : ⊢ᶜ[< i] Δ) (f : ℕ → SyntacticTerm L) :
+    ⊢ᶜ[< i] Δ.map ((Rew.rewrite f).hom) := d.rewrite (by simp) f
 
-def rewriteCut {Δ : Sequent L} (d : ⊢ᶜ Δ) (f : ℕ → SyntacticTerm L) : ⊢ᶜ Δ.image ((Rew.rewrite f).hom) := d.rewrite (by simp) f
+def rewriteCut {Δ : Sequent L} (d : ⊢ᶜ Δ) (f : ℕ → SyntacticTerm L) :
+    ⊢ᶜ Δ.map ((Rew.rewrite f).hom) := d.rewrite (by simp) f
 
-@[simp] lemma length_rewrite (h) (d : ⊢ᶜ[P] Δ) (f : ℕ → SyntacticTerm L) : (d.rewrite h f).length = d.length :=
-  by induction d generalizing f <;> simp[*, DerivationCR.rewrite]
+@[simp] lemma length_rewrite (h) (d : ⊢ᶜ[P] Δ) (f : ℕ → SyntacticTerm L) :
+    (d.rewrite h f).length = d.length := by
+  induction d generalizing f <;> simp[*, DerivationCR.rewrite, -List.map_cons]
+  case axL => rw[length_cast] <;> simp[Rew.rel, Rew.nrel]
+  case all => rw[length_cast] <;> simp[Rew.q_rewrite, *]
+  case ex => rw[length_cast] <;> simp[Rew.q_rewrite, *]
 
 @[simp] lemma length_rewrite₀ (d : ⊢ᵀ Δ) (f : ℕ → SyntacticTerm L) : (d.rewrite₀ f).length = d.length :=
   d.length_rewrite _ f
 
 protected def map (h : ∀ f p, P p → P ((Rew.rewrite f).hom p)) {Δ : Sequent L} (d : ⊢ᶜ[P] Δ) (f : ℕ → ℕ) :
-    ⊢ᶜ[P] Δ.image (Rew.rewriteMap f).hom := d.rewrite h _
+    ⊢ᶜ[P] Δ.map (Rew.rewriteMap f).hom := d.rewrite h _
 
-protected def shift (h : ∀ f p, P p → P ((Rew.rewrite f).hom p)) {Δ : Sequent L} (d : ⊢ᶜ[P] Δ) : ⊢ᶜ[P] (shifts Δ) :=
-  (d.map h Nat.succ).cast (by simp[shifts_eq_image]; congr)
+protected def shift (h : ∀ f p, P p → P ((Rew.rewrite f).hom p)) {Δ : Sequent L} (d : ⊢ᶜ[P] Δ) :
+    ⊢ᶜ[P] Δ⁺ :=
+  (d.map h Nat.succ).cast (by simp[shifts]; congr)
 
 private lemma map_subst_eq_free (p : SyntacticSubformula L 1) (h : ¬p.fvar? m) :
-    (Rew.rewriteMap (fun x => if x = m then 0 else x + 1)).hom ([→ &m].hom p) = Rew.free.hom p := by
+    (Rew.rewriteMap (fun x => if x = m then 0 else x + 1)).hom (p/[&m]) = Rew.free.hom p := by
   simp[←Rew.hom_comp_app];
   exact Subformula.rew_eq_of_funEqOn (by simp[Rew.comp_app, Fin.eq_zero])
     (fun x hx => by simp[Rew.comp_app]; rintro rfl; contradiction)
 
-private lemma image_map₀_eq_shifts (Δ : Finset $ SyntacticFormula L) (h : ∀ p ∈ Δ, ¬p.fvar? m) :
-    Δ.image (Rew.rewriteMap (fun x => if x = m then 0 else x + 1)).hom = shifts Δ := by
-  simp[shifts_eq_image]; apply Finset.image_congr
+private lemma map_rewriteMap_eq_shifts (Δ : Sequent L) (h : ∀ p ∈ Δ, ¬p.fvar? m) :
+    Δ.map (Rew.rewriteMap (fun x => if x = m then 0 else x + 1)).hom = Δ⁺ := by
+  simp[shifts]; apply List.map_congr
   intro p hp; exact rew_eq_of_funEqOn₀ (by intro x hx; simp; rintro rfl; have := h p hp; contradiction)
 
-def genelalizeByNewver (h : ∀ f p, P p → P ((Rew.rewrite f).hom p)) {p : SyntacticSubformula L 1} (hp : ¬p.fvar? m) (hΔ : ∀ q ∈ Δ, ¬q.fvar? m)
-  (d : ⊢ᶜ[P] insert ([→ &m].hom p) Δ) : ⊢ᶜ[P] insert (∀' p) Δ := by
-  have : ⊢ᶜ[P] insert (Rew.free.hom p) (shifts Δ) :=
-    (d.map h (fun x => if x = m then 0 else x + 1)).cast (by simp[map_subst_eq_free p hp, image_map₀_eq_shifts Δ hΔ])
-  exact all Δ p this
+def genelalizeByNewver (h : ∀ f p, P p → P ((Rew.rewrite f).hom p))
+    {p : SyntacticSubformula L 1} (hp : ¬p.fvar? m) (hΔ : ∀ q ∈ Δ, ¬q.fvar? m)
+    (d : ⊢ᶜ[P] p/[&m] :: Δ) : ⊢ᶜ[P] (∀' p) :: Δ := by
+  have : ⊢ᶜ[P] (Rew.free.hom p) :: Δ⁺ :=
+    (d.map h (fun x => if x = m then 0 else x + 1)).cast
+    (by simp[map_subst_eq_free p hp, map_rewriteMap_eq_shifts Δ hΔ])
+  exact all this
 
 def genelalizeByNewver₀ {p : SyntacticSubformula L 1} (hp : ¬p.fvar? m) (hΔ : ∀ q ∈ Δ, ¬q.fvar? m)
-  (d : ⊢ᵀ insert ([→ &m].hom p) Δ) : ⊢ᵀ insert (∀' p) Δ := d.genelalizeByNewver (by simp) hp hΔ
+  (d : ⊢ᵀ p/[&m] :: Δ) : ⊢ᵀ (∀' p) :: Δ := d.genelalizeByNewver (by simp) hp hΔ
 
 def genelalizeByNewverCut {p : SyntacticSubformula L 1} (hp : ¬p.fvar? m) (hΔ : ∀ q ∈ Δ, ¬q.fvar? m)
-  (d : ⊢ᶜ insert ([→ &m].hom p) Δ) : ⊢ᶜ insert (∀' p) Δ := d.genelalizeByNewver (by simp) hp hΔ
+  (d : ⊢ᶜ p/[&m] :: Δ) : ⊢ᶜ (∀' p) :: Δ := d.genelalizeByNewver (by simp) hp hΔ
 
 def exOfInstances (v : List (SyntacticTerm L)) (p : SyntacticSubformula L 1)
-  (h : ⊢ᶜ[P] (v.map (fun t => (Rew.substs ![t]).hom p)).toFinset ∪ Γ) : ⊢ᶜ[P] insert (∃' p) Γ := by
+  (h : ⊢ᶜ[P] v.map (p/[·]) ++ Γ) : ⊢ᶜ[P] (∃' p) :: Γ := by
   induction' v with t v ih generalizing Γ <;> simp at h
-  · exact weakening h (Finset.subset_insert _ Γ)
-  · exact (ih (Γ := insert (∃' p) Γ)
-      ((ex _ t p h).cast (by ext r; simp))).cast (by simp)
+  · exact weakening h (List.subset_cons _ _)
+  · exact (ih (Γ := (∃' p) :: Γ)
+      ((ex t h).wk (by simp; exact List.subset_append_of_subset_right _ (List.subset_cons _ _)))).wk
+        (by simp)
 
 def exOfInstances' (v : List (SyntacticTerm L)) (p : SyntacticSubformula L 1)
-  (h : ⊢ᶜ[P] (insert (∃' p) $ (v.map (fun t => (Rew.substs ![t]).hom p)).toFinset ∪ Γ)) : ⊢ᶜ[P] insert (∃' p) Γ :=
-  (exOfInstances (Γ := insert (∃' p) Γ) v p (h.cast $ by simp)).cast (by simp)
+  (h : ⊢ᶜ[P] (∃' p) :: v.map (p/[·]) ++ Γ) : ⊢ᶜ[P] (∃' p) :: Γ :=
+  (exOfInstances (Γ := (∃' p) :: Γ) v p
+    (h.wk $ by simp; exact List.subset_append_of_subset_right _ (List.subset_cons _ _))).wk
+    (by simp)
+
+def toTait {Γ : List (Sentence L)} (d : ⊢ᶜ Γ.map Rew.emb.hom) : ⊢¹ Γ := d
+
+def ofTait {Γ : List (Sentence L)} (d : ⊢¹ Γ) : ⊢ᶜ Γ.map Rew.emb.hom := d
 
 end DerivationCR
 
-structure DerivationCRWA (P : SyntacticFormula L → Prop) (T : Theory L) (Δ : Sequent L) where
-  leftHand : Finset (Sentence L)
-  hleftHand : ↑leftHand ⊆ (~·) '' T
-  derivation : ⊢ᶜ[P] Δ ∪ (leftHand.image Rew.emb.hom)
+instance : Tait (Sentence L) where
+  verum := fun Δ =>
+    have d : ⊢ᶜ ⊤ :: Δ.map Rew.emb.hom := DerivationCR.verum (Δ.map Rew.emb.hom)
+    DerivationCR.toTait (d.cast $ by simp)
+  and := fun {σ π Δ} dσ dπ =>
+    let dσ : ⊢ᶜ Rew.emb.hom σ :: Δ.map Rew.emb.hom := DerivationCR.ofTait dσ
+    let dπ : ⊢ᶜ Rew.emb.hom π :: Δ.map Rew.emb.hom := DerivationCR.ofTait dπ
+    DerivationCR.toTait ((dσ.and dπ).cast $ by simp)
+  or := fun {σ π Δ} d =>
+    let d : ⊢ᶜ Rew.emb.hom σ :: Rew.emb.hom π :: Δ.map Rew.emb.hom := DerivationCR.ofTait d
+    DerivationCR.toTait (d.or.cast $ by simp)
+  wk := fun {Δ Δ'} d ss =>
+    d.wk (List.map_subset _ ss)
+  em := fun {σ Δ} hp hn =>
+    DerivationCR.toTait
+      (DerivationCR.em (p := Rew.emb.hom σ)
+        (List.mem_map_of_mem _ hp) (by simpa using List.mem_map_of_mem Rew.emb.hom hn))
 
-scoped notation :45 T " ⊢ᶜ[" P "] " Γ:45 => DerivationCRWA P T Γ
-
-abbrev DerivationWA (T : Theory L) (Δ : Sequent L) := DerivationCRWA (fun _ => False) T Δ
-
-scoped infix:45 " ⊢ᵀ " => DerivationWA
-
-abbrev DerivationCWA (T : Theory L) (Δ : Sequent L) := DerivationCRWA (fun _ => True) T Δ
-
-scoped infix:45 " ⊢' " => DerivationCWA
-
-instance Proof : System (Sentence L) where
-  Bew := fun T σ => T ⊢' {Rew.emb.hom σ}
-  axm := fun {f σ} hσ =>
-    { leftHand := {~σ}
-      hleftHand := by simp[hσ]
-      derivation := DerivationCR.em (p := Rew.emb.hom σ) (by simp) (by simp) }
-  weakening' := fun {T U} f h b =>
-    { leftHand := b.leftHand,
-      hleftHand := Set.Subset.trans b.hleftHand (Set.image_subset _ h),
-      derivation := b.derivation }
-
-def DerivationCRWA.toDerivationCWA {T : Theory L} {Δ} (b : T ⊢ᶜ[P] Δ) : T ⊢' Δ where
-  leftHand := b.leftHand
-  hleftHand := b.hleftHand
-  derivation := b.derivation.cutWeakening (by simp)
-
-def DerivationCWA.toDerivationCWA {T : Theory L} {σ : Sentence L} (b : T ⊢ σ) : T ⊢' {Rew.emb.hom σ} := b
-
-def DerivationCRWA.toProof {T : Theory L} {σ : Sentence L} (b : T ⊢ᶜ[P] {Rew.emb.hom σ}) : T ⊢ σ :=
-  b.toDerivationCWA
-
-def DerivationCWA.toDerivationWA {T : Theory L} {σ : Sentence L} (b : T ⊢ σ) : T ⊢' {Rew.emb.hom σ} := b
-
-def DerivationCR.toDerivationCRWA
-  {P : SyntacticFormula L → Prop} (T : Theory L) {Δ : Sequent L} (b : ⊢ᶜ[P] Δ) : T ⊢ᶜ[P] Δ where
-  leftHand := ∅
-  hleftHand := by simp
-  derivation := b.cast (by simp)
-
-namespace DerivationCRWA
-
-variable {P : SyntacticFormula L → Prop} {T : Theory L} {Δ : Sequent L}
-
-def kernel (b : DerivationCRWA P T Δ) := b.leftHand.image (~·)
-
-lemma neg_mem {b : T ⊢ᶜ[P] Δ} (hσ : σ ∈ b.leftHand) : ~σ ∈ T := by
-  have : ∃ q ∈ T, ~q = σ := b.hleftHand hσ; rcases this with ⟨q, hq, rfl⟩; simp[hq]
-
-@[simp] lemma kernel_subset (b : T ⊢ᶜ[P] Δ) : ↑(b.kernel) ⊆ T := by
-  simp[kernel]; intros p hp; exact neg_mem hp
-
-lemma compact {p} (b : T ⊢ᶜ[P] p) : b.kernel ⊢ᶜ[P] p where
-  leftHand := b.leftHand
-  hleftHand := by simp[kernel, ←Set.image_comp]
-  derivation := b.derivation
-
-def verum (h : ⊤ ∈ Δ) : T ⊢ᶜ[P] Δ := (DerivationCR.verum _ (by simp[h])).toDerivationCRWA T
-
-def axL {k} (r : L.Rel k) (v : Fin k → SyntacticTerm L) (h : rel r v ∈ Δ) (nh : nrel r v ∈ Δ) : T ⊢ᶜ[P] Δ :=
-  (DerivationCR.axL Δ r v h nh).toDerivationCRWA T
-
-protected def and {p₁ p₂} (h : p₁ ⋏ p₂ ∈ Δ) (b₁ : T ⊢ᶜ[P] insert p₁ Δ) (b₂ : T ⊢ᶜ[P] insert p₂ Δ) :
-    T ⊢ᶜ[P] Δ where
-  leftHand := b₁.leftHand ∪ b₂.leftHand
-  hleftHand := by simp[b₁.hleftHand, b₂.hleftHand]
-  derivation :=
-    let d : ⊢ᶜ[P] insert (p₁ ⋏ p₂) (Δ ∪ (b₁.leftHand ∪ b₂.leftHand).image Rew.emb.hom) :=
-      DerivationCR.and (Δ ∪ (b₁.leftHand ∪ b₂.leftHand).image Rew.emb.hom) p₁ p₂
-        (b₁.derivation.weakening (by intro x; simp; rintro (rfl | hx | ⟨σ, hσ, rfl⟩); { simp }; { simp[hx] }; { exact Or.inr $ Or.inr ⟨σ, Or.inl hσ, rfl⟩ } ))
-        (b₂.derivation.weakening (by intro x; simp; rintro (rfl | hx | ⟨σ, hσ, rfl⟩); { simp }; { simp[hx] }; { exact Or.inr $ Or.inr ⟨σ, Or.inr hσ, rfl⟩ } ))
-    d.cast (Finset.insert_eq_of_mem (by simp[h]))
-
-protected def or {p₁ p₂} (h : p₁ ⋎ p₂ ∈ Δ) (b : T ⊢ᶜ[P] insert p₁ (insert p₂ Δ)) : T ⊢ᶜ[P] Δ where
-  leftHand := b.leftHand
-  hleftHand := b.hleftHand
-  derivation :=
-    let d : ⊢ᶜ[P] insert (p₁ ⋎ p₂) (Δ ∪ b.leftHand.image Rew.emb.hom) :=
-      DerivationCR.or (Δ ∪ b.leftHand.image Rew.emb.hom) p₁ p₂ (b.derivation.cast (by simp[Finset.insert_union]))
-    d.cast (Finset.insert_eq_of_mem (by simp[h]))
-
-protected def all {p} (h : ∀' p ∈ Δ)
-  (b : T ⊢ᶜ[P] (insert (Rew.free.hom p) (shifts Δ))) : T ⊢ᶜ[P] Δ where
-  leftHand := b.leftHand
-  hleftHand := b.hleftHand
-  derivation :=
-    let d₁ : ⊢ᶜ[P] insert (Rew.free.hom p) (shifts $ Δ ∪ b.leftHand.image Rew.emb.hom) := b.derivation.cast (by simp[shifts_union])
-    let d₂ : ⊢ᶜ[P] insert (∀' p) (Δ ∪ b.leftHand.image Rew.emb.hom):= d₁.all
-    d₂.cast (Finset.insert_eq_of_mem $ by simp[h])
-
-protected def ex {p} {t} (h : ∃' p ∈ Δ)
-  (b : T ⊢ᶜ[P] (insert ([→ t].hom p) Δ)) : T ⊢ᶜ[P] Δ where
-  leftHand := b.leftHand
-  hleftHand := b.hleftHand
-  derivation :=
-    let d₁ : ⊢ᶜ[P] insert ([→ t].hom p) (Δ ∪ b.leftHand.image Rew.emb.hom) := by simpa using b.derivation
-    let d₂ : ⊢ᶜ[P] insert (∃' p) (Δ ∪ b.leftHand.image Rew.emb.hom) := DerivationCR.ex _ t p d₁
-    d₂.cast (Finset.insert_eq_of_mem $ by simp[h])
-
-protected def id {σ} (hσ : σ ∈ T) (b : T ⊢ᶜ[P] insert (~Rew.emb.hom σ) Δ) : T ⊢ᶜ[P] Δ where
-  leftHand := insert (~σ) b.leftHand
-  hleftHand := by simp[Set.insert_subset_iff, b.hleftHand, hσ]
-  derivation := b.derivation.cast (by ext ; simp)
-
-def cast {Δ₁ Δ₂ : Sequent L} (h : Δ₁ = Δ₂) (b : T ⊢ᶜ[P] Δ₁) : T ⊢ᶜ[P] Δ₂ := by rw[h] at b; exact b
-
-def weakeningRight {Δ₁ Δ₂ : Sequent L} (h : Δ₁ ⊆ Δ₂) (b : T ⊢ᶜ[P] Δ₁) : T ⊢ᶜ[P] Δ₂ where
-  leftHand := b.leftHand
-  hleftHand := b.hleftHand
-  derivation := b.derivation.weakening (Finset.union_subset_union_left h)
-
-def weakeningLeft {T U : Theory L} (h : T ⊆ U) (b : T ⊢ᶜ[P] Δ) : U ⊢ᶜ[P] Δ where
-  leftHand := b.leftHand
-  hleftHand := Set.Subset.trans b.hleftHand (Set.image_subset _ h)
-  derivation := b.derivation
-
-def deduction {σ} (b : insert σ T ⊢ᶜ[P] Δ) : T ⊢ᶜ[P] insert (~Rew.emb.hom σ) Δ where
-  leftHand := Finset.erase b.leftHand (~σ)
-  hleftHand := by simp; exact subset_trans b.hleftHand (by simp; intro σ; simp)
-  derivation := b.derivation.weakening
-    (by rw[Finset.insert_union, ←Finset.union_insert, Finset.image_erase (f := Rew.emb.hom) Rew.emb.hom_Injective]
-        simp[-Finset.insert_union, -Finset.union_insert]
-        exact Finset.union_subset_union_right (Finset.insert_erase_subset _ _))
-
-def resolution {σ} (b : T ⊢ᶜ[P] insert (Rew.emb.hom σ) Δ) : insert (~σ) T ⊢ᶜ[P] Δ where
-  leftHand := insert σ b.leftHand
-  hleftHand := by simp[Set.image_insert_eq]; exact Set.insert_subset_insert b.hleftHand
-  derivation := b.derivation.cast (by rw[Finset.insert_union, ←Finset.union_insert, Finset.image_insert])
-
-def elimFalsum (b : T ⊢ᶜ[P] Δ) : T ⊢ᶜ[P] Δ.erase ⊥ where
-  leftHand := b.leftHand
-  hleftHand := b.hleftHand
-  derivation :=
-    b.derivation.elimFalsum.weakening (by simp[Finset.erase_union_distrib]; exact Finset.union_subset_union_right (Finset.erase_subset _ _))
-
-def byAxiom {σ} (hσ : σ ∈ T) (h : Rew.emb.hom σ ∈ Δ) : T ⊢ᶜ[P] Δ where
-  leftHand := {~σ}
-  hleftHand := by simp[hσ]
-  derivation := DerivationCR.em (p := Rew.emb.hom σ) (by simp[h]) (by simp)
-
-protected def em {p} (hp : p ∈ Δ) (hn : ~p ∈ Δ) : T ⊢ᶜ[P] Δ := (DerivationCR.em hp hn).toDerivationCRWA T
-
-def and' {p₁ p₂} (b₁ : T ⊢ᶜ[P] insert p₁ Δ) (b₂ : T ⊢ᶜ[P] insert p₂ Δ) : T ⊢ᶜ[P] insert (p₁ ⋏ p₂) Δ :=
-  let b₁' : T ⊢ᶜ[P] insert p₁ (insert (p₁ ⋏ p₂) Δ) := b₁.weakeningRight (by simp[Finset.Insert.comm p₁, Finset.subset_insert])
-  let b₂' : T ⊢ᶜ[P] insert p₂ (insert (p₁ ⋏ p₂) Δ) := b₂.weakeningRight (by simp[Finset.Insert.comm p₂, Finset.subset_insert])
-  b₁'.and (by simp) b₂'
-
-def or' {p q} (b : T ⊢ᶜ[P] insert p (insert q Δ)) : T ⊢ᶜ[P] insert (p ⋎ q) Δ :=
-  let b' : T ⊢ᶜ[P] (insert p $ insert q $ insert (p ⋎ q) Δ) := b.weakeningRight (by simp[Finset.Insert.comm _ (p ⋎ q), Finset.subset_insert])
-  b'.or (by simp)
-
-def all' {p} (b : T ⊢ᶜ[P] insert (Rew.free.hom p) (shifts Δ)) : T ⊢ᶜ[P] insert (∀' p) Δ :=
-  let b' : T ⊢ᶜ[P] (insert (Rew.free.hom p) $ shifts $ insert (∀' p) Δ) :=
-    b.weakeningRight (by simp[Finset.Insert.comm (Rew.free.hom p), shifts_insert, Finset.subset_insert])
-  b'.all (by simp)
-
-def ex' {p} {t : SyntacticTerm L} (b : T ⊢ᶜ[P] insert ([→ t].hom p) Δ) : T ⊢ᶜ[P] insert (∃' p) Δ :=
-  let b' : T ⊢ᶜ[P] insert ([→ t].hom p) (insert (∃' p) Δ) :=
-    b.weakeningRight (by simp[Finset.Insert.comm ([→ t].hom p), shifts_insert, Finset.subset_insert])
-  b'.ex (by simp)
-
-def cCut {p} (b₁ : T ⊢' insert p Δ) (b₂ : T ⊢' insert (~p) Γ) : T ⊢' Δ ∪ Γ where
-  leftHand := b₁.leftHand ∪ b₂.leftHand
-  hleftHand := by simp[b₁.hleftHand, b₂.hleftHand]
-  derivation := by
-    have b₁' : ⊢ᶜ insert p (Δ ∪ b₁.leftHand.image Rew.emb.hom) := by simpa using b₁.derivation
-    have b₂' : ⊢ᶜ insert (~p) (Γ ∪ b₂.leftHand.image Rew.emb.hom) := by simpa using b₂.derivation
-    exact (b₁'.cCut b₂').cast (by simp only [←Finset.union_assoc, Finset.union_comm _ Γ, Finset.image_union])
-
-def cCut' {p} (b₁ : T ⊢' insert p Δ) (b₂ : T ⊢' insert (~p) Δ) : T ⊢' Δ := (b₁.cCut b₂).cast (by simp)
-
-protected def rewrite (f : ℕ → SyntacticTerm L) {T : Theory L} {Δ : Sequent L} (b : T ⊢' Δ) :
-    T ⊢' Δ.image ((Rew.rewrite f).hom) where
-  leftHand := b.leftHand
-  hleftHand := b.hleftHand
-  derivation := (b.derivation.rewriteCut f).cast
-    (by simp[Finset.image_union, Finset.image_image, Rew.hom_comp_eq]; congr; ext q; simp[←Rew.hom_comp_app])
-
-variable
-  {L₁ : Language} [∀ k, DecidableEq (L₁.Func k)] [∀ k, DecidableEq (L₁.Rel k)]
-  {L₂ : Language} [∀ k, DecidableEq (L₂.Func k)] [∀ k, DecidableEq (L₂.Rel k)]
-
-protected def lMap (Φ : L₁ →ᵥ L₂) {T : Theory L₁} {Δ : Sequent L₁} (b : T ⊢' Δ) :
-    Theory.lMap Φ T ⊢' Δ.image (Subformula.lMap Φ) where
-  leftHand := b.leftHand.image (Subformula.lMap Φ)
-  hleftHand := by
-    simp; intro σ hσ
-    have : ∃ τ ∈ T, ~τ = σ := by simpa using b.hleftHand hσ;
-    rcases this with ⟨τ, hτ, rfl⟩
-    simpa using Set.mem_image_of_mem _ hτ
-  derivation :=
-    (b.derivation.lMapCut Φ).cast
-    (by simp[Finset.image_union, Finset.image_image]; congr; ext x; simp[Subformula.lMap_emb])
-
-end DerivationCRWA
-
-theorem System.compact (T : Theory L) :
-    System.Consistent T ↔ ∀ T' : Finset (Sentence L), (T' : Theory L) ⊆ T → System.Consistent (T' : Theory L) :=
-  ⟨fun c u hu => c.of_subset hu, fun h => ⟨fun b => (h b.kernel (by simp)).false b.compact⟩⟩
-
-lemma consistent_iff_empty_sequent {T : Theory L} :
-    System.Consistent T ↔ IsEmpty (T ⊢' ∅) :=
-  ⟨by contrapose; simp[System.Consistent]; intro b; exact ⟨b.weakeningRight (by simp)⟩,
-   by contrapose; simp[System.Consistent]; intro b; exact ⟨b.elimFalsum.cast (by simp)⟩⟩
-
-lemma provable_iff_inConsistent {T : Theory L} :
-    Nonempty (T ⊢ σ) ↔ ¬System.Consistent (insert (~σ) T) :=
-  ⟨by rintro ⟨b⟩; simp[consistent_iff_empty_sequent]
-      have : T ⊢' insert (Rew.emb.hom σ) ∅ := b
-      exact ⟨this.resolution⟩,
-   by simp[consistent_iff_empty_sequent]; intro b
-      exact ⟨by simpa using b.deduction⟩⟩
-
-lemma inconsistent_of_provable_and_refutable {T : Theory L} {σ}
-  (bp : T ⊢ σ) (br : T ⊢ ~σ) : ¬System.Consistent T := fun A => by
-  have : T ⊢' ∅ := DerivationCRWA.cCut' bp (by simpa using DerivationCWA.toDerivationCWA br)
-  exact (consistent_iff_empty_sequent.mp A).false this
-
-lemma inconsistent_of_provable_and_refutable' {T : Theory L} {σ}
-    (bp : T ⊢! σ) (br : T ⊢! ~σ) : ¬System.Consistent T := by
-  rcases bp with ⟨bp⟩; rcases br with ⟨br⟩
-  exact inconsistent_of_provable_and_refutable bp br
-
-variable
-  {L₁ : Language} [∀ k, DecidableEq (L₁.Func k)] [∀ k, DecidableEq (L₁.Rel k)]
-  {L₂ : Language} [∀ k, DecidableEq (L₂.Func k)] [∀ k, DecidableEq (L₂.Rel k)]
-
-def System.lMap (Φ : L₁ →ᵥ L₂) {T : Theory L₁} {σ : Sentence L₁} (b : T ⊢ σ) :
-    Theory.lMap Φ T ⊢ Subformula.lMap Φ σ := by simpa[Subformula.lMap_emb] using b.lMap Φ
-
-lemma inConsistent_lMap (Φ : L₁ →ᵥ L₂) {T : Theory L₁} :
-    ¬System.Consistent T → ¬System.Consistent (Theory.lMap Φ T) := by
-  simp[System.Consistent]; intro b; exact ⟨by simpa using System.lMap Φ b⟩
-
-instance : Gentzen (Sentence L) where
-  Derivation := fun Γ Δ => ⊢ᶜ ((Γ.map (~Rew.emb.hom ·)).toFinset ∪ (Δ.map Rew.emb.hom).toFinset)
-  verum := fun _ _ => DerivationCR.verum _ (by simp)
-  falsum := fun _ _ => DerivationCR.verum _ (by simp)
-  negLeft := fun b => b.cast (by simp)
-  negRight := fun b => b.cast (by simp)
-  andLeft := fun b => by simpa using DerivationCR.or _ _ _ (by simpa using b)
-  andRight := fun bp bq => by simpa using DerivationCR.and _ _ _ (by simpa using bp) (by simpa using bq)
-  orLeft := fun bp bq => by simpa using DerivationCR.and _ _ _ (by simpa using bp) (by simpa using bq)
-  orRight := fun b => by simpa using DerivationCR.or _ _ _ (by simpa using b)
-  implyLeft := fun bp bq => by simpa[Subformula.imp_eq] using DerivationCR.and _ _ _ (by simpa using bp) (by simpa using bq)
-  implyRight := fun b => by simpa[Subformula.imp_eq] using DerivationCR.or _ _ _ (b.cast $ by simp[Finset.Insert.comm])
-  wk := fun b hΓ hΔ => b.weakening
-    (Finset.union_subset_union
-      (by simpa[List.toFinset_map] using Finset.image_subset_image (List.toFinset_mono hΓ))
-      (List.toFinset_mono $ List.map_subset _ hΔ))
-  em := fun {p} _ _ hΓ hΔ =>
-    DerivationCR.em (p := Rew.emb.hom p)
-      (by simp[*]; exact Or.inr ⟨p, hΔ, rfl⟩)
-      (by simp[*]; exact Or.inl ⟨p, hΓ, rfl⟩)
-
-
-variable {T : Theory L} {Γ Δ : List (Sentence L)}
-
-def gentzen_trans (hΓ : ∀ σ ∈ Γ, T ⊢ σ) (d : Γ ⊢ᴳ Δ) : T ⊢' (Δ.map Rew.emb.hom).toFinset := by
-  induction' Γ with σ Γ ih generalizing Δ
-  · exact (d.toDerivationCRWA T).cast (by simp)
-  · have d' : Γ ⊢ᴳ ~σ :: Δ := d.cast (by simp)
-    have b₁ : T ⊢' insert (Rew.emb.hom σ) ∅  := hΓ σ (by simp)
-    have b₂ : T ⊢' insert (~Rew.emb.hom σ) (Δ.map Rew.emb.hom).toFinset := by simpa using ih (fun p hp => hΓ p (by simp[hp])) d'
-    exact (b₁.cCut b₂).cast (by simp)
-
-instance : LawfulGentzen (Sentence L) where
-  toProof₁ := fun d h => DerivationCRWA.toProof (by simpa using gentzen_trans h d)
+instance : Tait.Cut (Sentence L) := ⟨fun {Δ σ} dp dn =>
+  DerivationCR.toTait (DerivationCR.cCut (p := Rew.emb.hom σ)
+    (DerivationCR.ofTait dp) ((DerivationCR.ofTait dn).cast $ by simp))⟩
 
 end FirstOrder
 
